WIP

src/tls/AEADProvider.fst
@@ -10,16 +10,9 @@ open FStar.UInt32
 
 module CC = CoreCrypto
 module OAEAD = AEADOpenssl
-module CAEAD = LowCProvider
-
-module Plain = Crypto.Plain
-module AE = Crypto.AEAD.Main
-module CB = Crypto.Symmetric.Bytes
 
 type provider =
   | OpenSSLProvider
-  | LowProvider
-  | LowCProvider
 
 let use_provider () : Tot provider =
   OpenSSLProvider
@@ -28,43 +21,6 @@ let debug = false
 let prov() =
   match use_provider() with
   | OpenSSLProvider -> "OpenSSLProvider"
-  | LowCProvider -> "LowCProvider"
-  | LowProvider -> "LowProvider"
-
-type u32 = FStar.UInt32.t
-
-(**
-Functions to go back and forth between Platform.Bytes Buffers
-**)
-#set-options "--z3rlimit 100 --initial_fuel 1 --max_fuel 1 --initial_ifuel 1 --max_ifuel 1"
-val to_bytes: l:nat -> buf:CB.lbuffer l -> STL (b:bytes{length b = l})
-  (requires (fun h0 -> Buffer.live h0 buf))
-  (ensures (fun h0 s h1 -> h0 == h1 ))
-let rec to_bytes l buf =
-  if l = 0 then empty_bytes
-  else
-    let b = Buffer.index buf 0ul in
-    let s = abyte b in
-    let t = to_bytes (l - 1) (Buffer.sub buf 1ul (uint_to_t (l-1))) in
-    let r = s @| t in
-    (lemma_len_append s t; r)
-
-#set-options "--z3rlimit 100 --initial_fuel 1 --max_fuel 1 --initial_ifuel 1 --max_ifuel 1"
-val store_bytes: len:nat -> buf:CB.lbuffer len -> i:nat{i <= len} -> b:bytes{length b = len} -> STL unit
-  (requires (fun h0 -> Buffer.live h0 buf))
-  (ensures (fun h0 r h1 -> Buffer.live h1 buf /\ Buffer.modifies_1 buf h0 h1))
-let rec store_bytes len buf i s =
-  if i < len then
-    let () = Buffer.upd buf (uint_to_t i) (Platform.Bytes.index s i) in
-    store_bytes len buf (i + 1) s
-
-val from_bytes: b:bytes{FStar.UInt.fits (length b) 32} -> StackInline (CB.lbuffer (length b))
-  (requires (fun h0 -> True))
-  (ensures (fun h0 r h1 -> Buffer.modifies_0 h0 h1 /\ Buffer.live h1 r ))
-let from_bytes b =
-  let buf = Buffer.create 0uy (uint_to_t (length b)) in
-  store_bytes (length b) buf 0 b;
-  buf
 
 (***********************************************************************)
 
@@ -110,9 +66,6 @@ type salt (i:id) = lbytes (salt_length i)
 
 noeq type state (i:id) (r:rw) =
 | OpenSSL: st:OAEAD.state i r -> salt:salt i -> state i r
-| LowC: st:CAEAD.aead_state -> key:key i -> salt:salt i -> state i r
-| LowLevel: 
-    st:AE.aead_state i (Crypto.Indexing.rw2rw r) -> salt: salt i -> state i r
 
 type writer i = s:state i Writer
 type reader i = s:state i Reader
@@ -130,9 +83,7 @@ let coerce_iv (i:id) (b:lbytes (iv_length i)) : Tot (iv i) = b
 let create_nonce (#i:id) (#rw:rw) (st:state i rw) (n:nonce i)
   : Tot (i:iv i) =
   let salt : salt i = match st with
-    | OpenSSL _ s -> s
-    | LowLevel _ s -> s
-    | LowC _ _ s -> s in
+    | OpenSSL _ s -> s in
   match (pv_of_id i, alg i) with
   | (TLS_1p3, _) | (_, CC.CHACHA20_POLY1305) ->
     xor (iv_length i) n salt
@@ -149,9 +100,7 @@ let lemma_nonce_iv (#i:id) (#rw:rw) (st:state i rw) (n1:nonce i) (n2:nonce i)
   : Lemma (create_nonce st n1 = create_nonce st n2 ==> n1 = n2)
   =
   let salt : salt i = match st with
-    | OpenSSL _ s -> s
-    | LowLevel _ s -> s
-    | LowC _ _ s -> s in
+    | OpenSSL _ s -> s in
   match (pv_of_id i, alg i) with
   | (TLS_1p3, _) | (_, CC.CHACHA20_POLY1305) ->
     lemma_xor_idempotent (iv_length i) n1 salt;
@@ -162,32 +111,19 @@ let lemma_nonce_iv (#i:id) (#rw:rw) (st:state i rw) (n1:nonce i) (n2:nonce i)
 
 type empty_log (#i:id) (#rw:rw) (st:state i rw) h =
   (match st with
-  | OpenSSL s _ -> OAEAD.empty_log s h
-  | LowC st _ _ -> True // TODO
-  | LowLevel st _ -> True) // TODO
+  | OpenSSL s _ -> OAEAD.empty_log s h) // TODO
 
 let region (#i:id) (#rw:rw) (st:state i rw) =
   (match st with
-  | OpenSSL st _ -> OAEAD.State?.region st
-  | LowC st _ _ -> tls_region // TODO
-  | LowLevel st _ -> tls_region) // TODO
+  | OpenSSL st _ -> OAEAD.State?.region st) // TODO
 
 let log_region (#i:id) (#rw:rw) (st:state i rw) =
   match st with
   | OpenSSL st _ -> OAEAD.State?.log_region st
-  | LowC st _ _ -> let r:rgn = tls_region in r // TODO
-  | LowLevel st _ -> let r:rgn = tls_region in r // TODO
-(*
-    assume(r<>root);
-    assume(forall (s:rid).{:pattern is_eternal_region s} is_above s r ==> is_eternal_region s);
-    r
-*)
 
 let st_inv (#i:id) (#rw:rw) (st:state i rw) h =
   match st with
   | OpenSSL st _ -> True
-  | LowC st _ _ -> True
-  | LowLevel st _ -> True // TODO
 
 let genPost (#i:id) (parent:rgn) h0 (w:writer i) h1 =
   modifies_none h0 h1 /\
@@ -206,15 +142,6 @@ let gen (i:id) (r:rgn) : ST (state i Writer)
   | OpenSSLProvider ->
     let st : OAEAD.state i Writer = OAEAD.gen r i in
     OpenSSL st salt
-  | LowCProvider ->
-    assume false; // TODO
-    let kv: key i = CC.random (CC.aeadKeySize (alg i)) in
-    let st = CAEAD.aead_create (alg i) CAEAD.ValeAES kv in
-    LowC st kv salt
-  | LowProvider ->
-    assume false; // TODO
-    let st = AE.gen i tls_region r in
-    LowLevel st salt
 
 let leak (#i:id) (#rw:rw) (st:state i rw)
   : ST (key i * salt i)
@@ -223,12 +150,6 @@ let leak (#i:id) (#rw:rw) (st:state i rw)
   =
   match st with
   | OpenSSL st s -> (OAEAD.leak st, s)
-  | LowC st k s -> (k, s)
-  | LowLevel st s ->
-    assume (false);
-    assume(~(Flag.prf i));
-    let k = AE.leak #i st in
-    (to_bytes (key_length i) k, s)
 
 // ADL TODO
 // There is an issue connecting the stateful encryption in miTLS
@@ -243,13 +164,6 @@ let genReader (parent:rgn) (#i:id) (st:writer i) : ST (reader i)
   | OpenSSL w salt ->
     // CoreCrypto state is in an external region
     OpenSSL (OAEAD.genReader parent w) salt
-  | LowLevel st salt ->
-    assume false;
-    let st' : AE.aead_state i Crypto.Indexing.Reader = AE.genReader st in
-    LowLevel st' salt
-  | LowC st k s ->
-    assume false;
-    LowC st k s
 
 let coerce (i:id) (r:rgn) (k:key i) (s:salt i)
   : ST (state i Writer)
@@ -260,12 +174,6 @@ let coerce (i:id) (r:rgn) (k:key i) (s:salt i)
     match use_provider() with
     | OpenSSLProvider ->
       OpenSSL (OAEAD.coerce r i k) s
-    | LowCProvider ->
-      let st = CAEAD.aead_create (alg i) CAEAD.ValeAES k in
-      LowC st k s
-    | LowProvider ->
-      let st = AE.coerce i r (from_bytes k) in
-      LowLevel st s
     in
   let r =
     if debug then
@@ -285,20 +193,9 @@ let taglen i = CC.aeadTagSize (alg i)
 let cipherlen i (l:plainlen) : n:nat{n >= taglen i} = l + taglen i
 type cipher i (l:plainlen) = lbytes (cipherlen i l)
 
-let uint128_of_iv (#i:id) (iv:iv i)
-  : Tot (n:FStar.UInt128.t{FStar.UInt128.v n < pow2 96})
-  =
-  let ivn = int_of_bytes iv in
-  assume(FStar.UInt.size ivn 128); // PROVEME need stronger post-condition on int_of_bytes
-  let iv128 = FStar.UInt128.uint_to_t ivn in
-  assume(FStar.UInt128.v iv128 < pow2 96); // PROVEME
-  iv128
-
 type fresh_iv (#i:id{authId i}) (w:writer i) (iv:iv i) h =
   (match w with
-  | OpenSSL st _ -> OAEAD.fresh_iv #i st iv h
-  | LowLevel st _ -> True // TODO
-  | _ -> True)
+  | OpenSSL st _ -> OAEAD.fresh_iv #i st iv h)
 
 let logged_iv (#i:id{authId i}) (#l:plainlen) (#rw:rw) (s:state i rw) (iv:iv i)
               (ad:adata i) (p:plain i l) (c:cipher i l) h =
@@ -317,32 +214,10 @@ let encrypt (#i:id) (#l:plainlen) (w:writer i) (iv:iv i) (ad:adata i) (plain:pla
     FStar.UInt.size (length ad) 32 /\ FStar.UInt.size l 32))
   (ensures (fun h0 cipher h1 -> modifies_one (log_region w) h0 h1))
   =
-  push_frame();
   let cipher =
     match w with
     | OpenSSL st _ -> OAEAD.encrypt st iv ad plain
-    | LowC st _ _ ->
-      assume(CAEAD.alg st = alg i); // assume val in the .fst
-      CAEAD.aead_encrypt st iv ad plain
-    | LowLevel st _ ->
-      let adlen = uint_to_t (length ad) in
-      let ad = from_bytes ad in
-      let plainlen = uint_to_t l in
-      let cipherlen = uint_to_t (cipherlen i l) in
-      assume(AE.safelen i (v plainlen) = true); // TODO
-      let plainbuf = from_bytes plain in
-      let plainba = CB.load_bytes plainlen plainbuf in
-      let plain = Plain.create i 0uy plainlen in
-      if not (Flag.safeId i) then begin
-        let pb = Plain.make #i l plainba in
-        Plain.store #i plainlen plain pb
-      end;
-      let cipher = Buffer.create 0uy cipherlen in
-      assume(v cipherlen = v plainlen + 12);
-      AE.encrypt i st (uint128_of_iv iv) adlen ad plainlen plain cipher;
-      to_bytes l cipher
   in
-  pop_frame ();
   cipher
 
   (*
@@ -371,18 +246,6 @@ let decrypt (#i:id) (#l:plainlen) (st:reader i) (iv:iv i) (ad:adata i) (cipher:c
   let plain =
     match st with
     | OpenSSL st _ -> OAEAD.decrypt st iv ad cipher
-    | LowC st _ _ -> CAEAD.aead_decrypt st iv ad cipher
-    | LowLevel st _->
-      let ivlen = uint_to_t (iv_length i) in
-      let iv = CB.load_uint128 ivlen (from_bytes iv) in
-      let adlen = uint_to_t (length ad) in
-      let ad = from_bytes ad in
-      let plainlen = uint_to_t l in
-      let cbuf = from_bytes cipher in
-      let plain = Plain.create i 0uy plainlen in
-      if AE.decrypt i st iv adlen ad plainlen plain cbuf then
-        Some (to_bytes l (Plain.bufferRepr #i plain))
-      else None
     in
   plain
 
@@ -408,28 +271,28 @@ let decrypt (#i:id) (#l:plainlen) (st:reader i) (iv:iv i) (ad:adata i) (cipher:c
 /// - for AEAD, we need a pair of algorithms for the cipher and for UFCMA---use Crypto.Indexing.fsti;
 /// - for StreamAE, we additionallly need the PV (to control the length of the static IV).
 ///
-/// We keep these parameters in AEADProvider and StreamAE instances, respectively. 
+/// We keep these parameters in AEADProvider and StreamAE instances, respectively.
 
 type aeadAlg // fixme.
 
 // TODO: add the two regions of AEAD.fsti, used only ideally (hence coerce is ~pure)
-type info (ip: ipkg) (aeadAlg_of_i: i:ip.IK.t -> aeadAlg) (i:ip.t) = a:aeadAlg {a = aeadAlg_of_i i} 
+type info (ip: ipkg) (aeadAlg_of_i: i:ip.IK.t -> aeadAlg) (i:ip.t) = a:aeadAlg {a = aeadAlg_of_i i}
 
 open IK
-unfold let localpkg 
-  (ip: ipkg) 
+unfold let localpkg
+  (ip: ipkg)
   (aeadAlg_of_i: i:ip.IK.t -> aeadAlg)
-  : 
+  :
   p: IK.local_pkg ip {IK.LocalPkg?.info #ip p == info1 ip ha_of_i good_of_i}
-= 
+=
     IK.LocalPkg
       (fun (i:ip.IK.t {ip.IK.registered i}) -> writer ip i)
       (info ip aeadAlg_of_i)
-      (fun #_ u -> aeadLen u) 
-      Flags.ideal_aead  
-      // local footprint 
+      (fun #_ u -> aeadLen u)
+      Flags.ideal_aead
+      // local footprint
       (fun #i (k:writer ip i) -> Set.empty (*17-11-24 regions for the PRF and the log *)  )
-      // local invariant 
+      // local invariant
       (fun #_ k h -> True)
       (fun r i h0 k h1 -> ())
       // create/coerce postcondition
