src/tls/Crypto.Plain.fsti
@@ -1,0 +1,11 @@
+module Crypto.Plain
+
+open Crypto.Indexing
+open Platform.Bytes
+open Flag
+
+type plainLen = nat
+val plain: i:id -> l:plainLen -> Type0
+val as_bytes: #i:id -> #l:plainLen -> p:plain i l -> GTot (lbytes l)
+val repr: #i:id {~(safeId i)} -> #l:plainLen -> p:plain i l -> Tot (b:lbytes l {b = as_bytes p })
+val make: #i:id {~(safeId i)}-> l:plainLen -> b:lbytes l -> Tot (p:plain i l {b = as_bytes p})
